progress on the unary example: proved up until the callback

theories/examples/stack_object_helpers.v
@@ -4,6 +4,49 @@ Require Import Eqdep_dec List.
 From cap_machine Require Import rules rules_LoadU_derived logrel fundamental region_invariants_revocation region_invariants_static region_invariants_batch_uninitialized.
 From cap_machine Require Export iris_extra addr_reg_sample region_macros contiguous stack_macros_helpers macros.
 
+(* TODO:move this to stdpp_extra *)
+Lemma elements_dom_list_to_map :
+      ∀ K V : Type,
+        EqDecision K → ∀ (EqDecision1 : EqDecision K) (H : Countable K) (l : list (K*V)),
+          NoDup (l.*1) →
+          elements (dom (gset K) (list_to_map l : gmap K V)) ≡ₚl.*1.
+Proof.
+  intros K V ? ? ? l Hdup. induction l.
+  - simpl. auto.
+  - destruct a as [k v]. simpl in *.
+    apply NoDup_cons in Hdup as [Hin Hdup].
+    rewrite dom_insert_L elements_union_singleton.
+    constructor. auto.
+    apply not_elem_of_dom.
+    apply not_elem_of_list_to_map_1. auto.
+Qed.
+
+Lemma elements_dom_list_to_map_zip :
+      ∀ K V : Type,
+        EqDecision K → ∀ (EqDecision1 : EqDecision K) (H : Countable K) (l1 : list K) (l2 : list V),
+          length l1 <= length l2 →
+          NoDup l1 →
+          elements (dom (gset K) (list_to_map (zip l1 l2) : gmap K V)) ≡ₚl1.
+Proof.
+  intros K V ? ? ? l1. induction l1.
+  - simpl. auto.
+  - intros l2 Hlen Hdup. destruct l2; [simpl in *; inversion Hlen|]. simpl in *.
+    apply NoDup_cons in Hdup as [Hin Hdup].
+    rewrite dom_insert_L elements_union_singleton.
+    constructor. apply IHl1; auto. lia.
+    apply not_elem_of_dom.
+    apply not_elem_of_list_to_map_1. rewrite fst_zip;auto. lia.
+Qed.
+
+Lemma Permutation_disjoint {A : Type} {eq1 : EqDecision A} {a : A} (l1 l2 l3 : list A) :
+  l1 ≡ₚl2 → l1 ## l3 -> l2 ## l3.
+Proof.
+  intros Hperm Hdisj.
+  apply elem_of_disjoint.
+  intros x Hx Hx'. revert Hx; rewrite -Hperm =>Hx.
+  apply elem_of_disjoint in Hdisj. apply Hdisj in Hx. done.
+Qed.
+
 Section stack_object.
   Context {Σ:gFunctors} {memg:memG Σ} {regg:regG Σ}
           {stsg : STSG Addr region_type Σ} {heapg : heapG Σ}
@@ -15,6 +58,32 @@ Section stack_object.
   Notation WORLD := (prodO STS_STD STS).
   Implicit Types W : WORLD.
 
+  (* TODO:move this to multiple_updates *)
+  Lemma std_update_multiple_disjoint W l1 l2 ρ1 ρ2 :
+    l1 ## l2 →
+    std_update_multiple (std_update_multiple W l2 ρ2) l1 ρ1 =
+    std_update_multiple (std_update_multiple W l1 ρ1) l2 ρ2.
+  Proof.
+    induction l1; intros Hdisj.
+    - simpl. auto.
+    - simpl. apply disjoint_cons in Hdisj as Hnin.
+      apply disjoint_weak in Hdisj.
+      apply IHl1 in Hdisj. rewrite Hdisj.
+      rewrite std_update_multiple_insert_commute;auto.
+  Qed.
+
+  Lemma region_addrs_disjoint_skip_middle b a2 a3 aend e :
+    (a2 + 1)%a = Some a3 → (a3 <= aend)%a →
+    region_addrs b a2 ++ region_addrs a3 aend ## [a2] ++ region_addrs aend e.
+  Proof.
+    intros Hsome Hle.
+    simpl. apply elem_of_disjoint.
+    intros x Hx Hx'.
+    apply elem_of_cons in Hx' as [-> | Hx'].
+    - apply elem_of_app in Hx as [Hx%elem_of_region_addrs | Hx%elem_of_region_addrs];solve_addr.
+    - apply elem_of_region_addrs in Hx'.
+      apply elem_of_app in Hx as [Hx%elem_of_region_addrs | Hx%elem_of_region_addrs];try solve_addr.
+  Qed.
 
   (* The following lemma will be used to make sure that any object passed as a parameter *)
   (* on the stack, will be disjoint from the current stack *)
@@ -147,6 +216,181 @@ Section stack_object.
     apply Forall_forall. intros x [k Hx]%elem_of_list_lookup. eapply Hforall. eauto.
   Qed.
 
+  (* After checking that the input stack object is all ints, we may need to re initialize it *)
+  (* For this purpose we will need to define a merge operation for "conditionally" closing the world *)
+  Fixpoint initialize_list l := λ W,
+    match l with
+    | [] => W
+    | a :: l' => match W.1 !! a with
+               | Some (Uninitialized _) => <s[a:=Monotemporary]s>(initialize_list l' W)
+               | _ => initialize_list l' W
+               end
+    end.
+
+  Lemma initialize_list_nin W l a :
+    a ∉ l → (initialize_list l W).1 !! a = W.1 !! a.
+  Proof.
+    intros Hnin.
+    induction l.
+    - simpl;auto.
+    - simpl. apply not_elem_of_cons in Hnin as [Hne Hnin].
+      rewrite -IHl;auto. destruct (W.1 !! a0);auto.
+      destruct r;auto. rewrite lookup_insert_ne//.
+  Qed.
+
+  Lemma initialize_list_perm W l a :
+    W.1 !! a = Some Permanent → (initialize_list l W).1 !! a = W.1 !! a.
+  Proof.
+    intros Hnin.
+    induction l.
+    - simpl;auto.
+    - simpl. destruct (decide (a0 = a));subst.
+      + rewrite Hnin;auto. rewrite IHl. auto.
+      + destruct (W.1 !! a0);auto. destruct r;auto. rewrite lookup_insert_ne//.
+  Qed.
+
+  Lemma initialize_list_in W l a w :
+    a ∈ l → W.1 !! a = Some (Uninitialized w) → (initialize_list l W).1 !! a = Some Monotemporary.
+  Proof.
+    intros Hin Huninit.
+    induction l;[inversion Hin|].
+    simpl. apply elem_of_cons in Hin as [-> | Hin].
+    - rewrite Huninit lookup_insert. auto.
+    - destruct (W.1 !! a0);auto. destruct r;auto.
+      destruct (decide (a = a0));subst;[rewrite lookup_insert|rewrite lookup_insert_ne//];auto.
+  Qed.
+
+
+
+  Lemma close_stack_object_mid W E m la1 la2 ρ wps l p bsec esec asec lsec :
+    (bsec <= asec)%a →
+    lsec = region_addrs asec esec →
+    length (region_addrs bsec esec) = length wps →
+    Forall (λ w : (Z + Cap) * Perm, ∃ z : Z, w.1 = inl z) wps →
+    Forall (λ awp : Addr * (Word * Perm),
+                    (uninitialize W m).1 !! awp.1 = Some Permanent ∨ (uninitialize W m).1 !! awp.1 = Some (Uninitialized awp.2.1))
+           (zip (region_addrs bsec esec) wps) →
+
+    region_addrs bsec esec ## (la1 ++ la2) →
+
+    region_conditions W l p bsec esec -∗
+    sts_full_world (std_update_multiple (std_update_multiple (uninitialize W m) la1 ρ) la2 Revoked) -∗
+    region (std_update_multiple (std_update_multiple (uninitialize W m) la1 ρ) la2 Revoked) ={E}=∗
+
+    sts_full_world (initialize_list lsec (std_update_multiple (std_update_multiple (uninitialize W m) la1 ρ) la2 Revoked)) ∗
+    region (initialize_list lsec (std_update_multiple (std_update_multiple (uninitialize W m) la1 ρ) la2 Revoked)).
+  Proof.
+    iIntros (Hle Heq Hlen Hints Hwps Hdisj) "#Hcond Hsts Hr".
+    iInduction (lsec) as [|a lsec] "IH" forall (asec Heq Hle).
+    - iModIntro. iSimpl. iFrame.
+    - assert (asec < esec)%a as Hlt.
+      { destruct (decide (esec <= asec))%a;[|solve_addr]. apply region_addrs_empty in l0. rewrite l0 in Heq. inversion Heq. }
+      rewrite region_addrs_cons // in Heq.
+      destruct (asec + 1)%a eqn:Hasec;[|exfalso;solve_addr].
+      simpl in Heq. assert (a = asec) as Heqa;[inversion Heq;auto|subst a].
+      assert (asec ∈ region_addrs bsec esec) as Hin.
+      { apply elem_of_region_addrs. solve_addr. }
+      apply elem_of_disjoint in Hdisj as Hlookup.
+      apply Hlookup in Hin as Hnin. apply not_elem_of_app in Hnin as [Hnin1 Hnin2].
+      rewrite /= std_sta_update_multiple_lookup_same_i// std_sta_update_multiple_lookup_same_i//.
+      assert (∃ wp, (asec,wp) ∈ zip (region_addrs bsec esec) wps) as [wp Hinwp].
+      { apply elem_of_list_lookup in Hin as [k Hk].
+        assert ((zip (region_addrs bsec esec) wps).*1 !! k = Some asec).
+        { rewrite fst_zip;[|lia]. auto. }
+        apply list_lookup_fmap_inv in H0 as [ [a' wp] [Hsubst Hy] ]. inversion Hsubst;subst.
+        exists wp. apply elem_of_list_lookup;eauto. }
+      revert Hwps; rewrite Forall_forall =>Hwps. apply Hwps in Hinwp as Hstate. simpl in Hstate.
+      destruct Hstate as [Hperm | Huninit].
+      + (* If the address is permanent, the world will not change *)
+        rewrite Hperm. iMod ("IH" $! a0 with "[] [] Hsts Hr") as "[$ $]". inversion Heq;auto. iPureIntro;solve_addr. auto.
+      + (* If the address is uninitialized, we need to reinitialise it using the ints assumption *)
+        rewrite Huninit. iMod ("IH" $! a0 with "[] [] Hsts Hr") as "[Hsts Hr]". inversion Heq;auto. iPureIntro;solve_addr.
+        (* get the read_write condition for asec *)
+        iDestruct (big_sepL_elem_of with "Hcond") as (p' Hflows) "[Hrel Hasec]";[apply Hin|].
+        assert (asec ∉ lsec) as Hnin.
+        { inversion Heq. intros Hcontr%elem_of_region_addrs. solve_addr. }
+        (* open the world to get the resource *)
+        iDestruct (region_open_uninitialized with "[$Hr $Hsts $Hrel]") as "(Hr & Hsts & Hstate & Hl & %)".
+        { rewrite initialize_list_nin// std_sta_update_multiple_lookup_same_i// std_sta_update_multiple_lookup_same_i//. }
+        (* assert that wp.1 is an int *)
+        apply elem_of_zip_r in Hinwp.
+        revert Hints;rewrite Forall_forall =>Hints. apply Hints in Hinwp as [z Hz].
+        destruct wp as [w p0]. simpl in Hz. subst w. simpl.
+        (* we can now close the world again and update its state to temp *)
+        destruct (pwl p') eqn:Hpwl.
+        * iMod (region_close_mono_uninit_w_pwl with "[$Hr $Hsts $Hstate $Hl $Hrel]") as "[$ $]";auto.
+          iSplit;auto. iSimpl. iSplit.
+          iModIntro. iIntros (W0 W' Hrelated) "_ /=". rewrite fixpoint_interp1_eq. eauto.
+          iNext. rewrite fixpoint_interp1_eq;eauto.
+        * iMod (region_close_mono_uninit_w_nwl with "[$Hr $Hsts $Hstate $Hl $Hrel]") as "[$ $]";auto.
+          iSplit;auto. iSimpl. iSplit.
+          iModIntro. iIntros (W0 W' Hrelated) "_ /=". rewrite fixpoint_interp1_eq. eauto.
+          iNext. rewrite fixpoint_interp1_eq;eauto.
+  Qed.
+
+  Lemma uninitialize_std_sta_lookup_perm :
+    ∀ (i : Addr) (m : Mem) (fs : STS_STD), fs !! i = Some Permanent <-> uninitialize_std_sta m fs !! i = Some Permanent.
+  Proof.
+    intros i m fs. split;intros Hperm.
+    - rewrite uninitialize_std_sta_spec Hperm.
+      destruct (m !! i);auto.
+    - rewrite uninitialize_std_sta_spec in Hperm.
+      destruct (fs !! i);auto. destruct (m !! i); auto.
+      inversion Hperm. destruct r;inversion H1. auto.
+  Qed.
+
+  Lemma close_stack_object W E m la1 la2 ρ wps l p bsec esec asec :
+    (if pwl l then p = Monotone else True) →
+    readAllowed l →
+    length (region_addrs bsec esec) = length wps →
+    Forall (λ w : (Z + Cap) * Perm, ∃ z : Z, w.1 = inl z) wps →
+    Forall (λ awp : Addr * (Word * Perm),
+                    (uninitialize W m).1 !! awp.1 = Some Permanent ∨ (uninitialize W m).1 !! awp.1 = Some (Uninitialized awp.2.1))
+           (zip (region_addrs bsec esec) wps) →
+
+    region_addrs bsec esec ## (la1 ++ la2) →
+
+    region_conditions W l p bsec esec -∗
+    sts_full_world (std_update_multiple (std_update_multiple (uninitialize W m) la1 ρ) la2 Revoked) -∗
+    region (std_update_multiple (std_update_multiple (uninitialize W m) la1 ρ) la2 Revoked) ={E}=∗
+
+    sts_full_world (initialize_list (region_addrs bsec esec) (std_update_multiple (std_update_multiple (uninitialize W m) la1 ρ) la2 Revoked)) ∗
+    region (initialize_list (region_addrs bsec esec) (std_update_multiple (std_update_multiple (uninitialize W m) la1 ρ) la2 Revoked)) ∗
+    interp (initialize_list (region_addrs bsec esec) (std_update_multiple (std_update_multiple (uninitialize W m) la1 ρ) la2 Revoked)) (inr (l, p, bsec, esec, asec)).
+  Proof.
+    iIntros (Hmono Hra Hlen Hints Hwps Hdisj) "#Hcond Hsts Hr".
+    iMod (close_stack_object_mid with "Hcond Hsts Hr") as "[$ $]";eauto. solve_addr.
+    iModIntro. rewrite fixpoint_interp1_eq /=.
+    assert (forall k y, region_addrs bsec esec !! k = Some y → ∃ wp, (y,wp) ∈ zip (region_addrs bsec esec) wps) as Hinwp.
+    { intros k y Hlook.
+      assert ((zip (region_addrs bsec esec) wps).*1 !! k = Some y).
+      { rewrite fst_zip;[|lia]. auto. }
+      apply list_lookup_fmap_inv in H0 as [ [a' wp] [Hsubst Hy] ]. inversion Hsubst;subst.
+      exists wp. apply elem_of_list_lookup;eauto. }
+    destruct l;inversion Hra.
+    3,6: destruct p;inversion Hmono.
+    all: try iApply (big_sepL_mono with "Hcond").
+    all: iIntros (k y Hk) "Hres /=".
+    all: iDestruct "Hres" as (p' Hflows) "(Hrel & %)".
+    all: iExists p';iFrame;iSplit;auto.
+    all: revert Hwps;rewrite Forall_forall =>Hwps.
+    all: assert (y ∈ region_addrs bsec esec) as Hy;[apply elem_of_list_lookup;eauto|].
+    all: apply Hinwp in Hk as [ [w p0] Hiny].
+    all: apply Hwps in Hiny; simpl in Hiny.
+    all: apply elem_of_disjoint in Hdisj.
+    all: apply Hdisj in Hy as Hny;apply not_elem_of_app in Hny as [Hy1 Hy2].
+    all: rewrite /region_state_nwl /region_state_pwl_mono.
+    1,2,5,6: destruct p;simpl in *.
+    all: try (apply uninitialize_std_sta_lookup_perm with (m:=m) in H0).
+    all: try (rewrite initialize_list_perm;by rewrite std_sta_update_multiple_lookup_same_i// std_sta_update_multiple_lookup_same_i//).
+    5,6: destruct Hiny as [Hiny | Hiny];
+      [apply uninitialize_std_sta_lookup_perm in Hiny; congruence
+      |rewrite (initialize_list_in _ _ _ w)// std_sta_update_multiple_lookup_same_i// std_sta_update_multiple_lookup_same_i//].
+    all: destruct Hiny as [Hiny | Hiny];
+      [iRight;rewrite initialize_list_perm// std_sta_update_multiple_lookup_same_i// std_sta_update_multiple_lookup_same_i//
+      |iLeft;rewrite (initialize_list_in _ _ _ w)// std_sta_update_multiple_lookup_same_i// std_sta_update_multiple_lookup_same_i//].
+  Qed.
+
   Lemma uninitialize_revoke_condition W m :
     (∀ a' : Addr, is_Some (m !! a') ↔ std W !! a' = Some Monotemporary ∧ (0 <= a')%a) →
     revoke_condition (uninitialize W m).
@@ -159,5 +403,18 @@ Section stack_object.
       intros Hcontr. assert (is_Some (m !! a)) as [? HisSome];[|congruence].
       apply Hforall. split;auto. solve_addr.
   Qed.
+
+  Lemma read_allowedU_inv_range W p g b e a b' e' :
+    (b <= b' ∧ e' < e)%a → readAllowedU p = true →
+    interp W (inr (p,g,b,e,a)) -∗
+    [∗ list] a ∈ region_addrs b' e', ∃ p', ⌜PermFlows (promote_perm p) p'⌝ ∗ read_write_cond a p' interp.
+  Proof.
+    iIntros ([Hle Hlt] HraU) "Hv".
+    iApply big_sepL_forall. iIntros (k x Hin).
+    assert (x ∈ region_addrs b' e') as [Hle' Hlt']%elem_of_region_addrs.
+    { apply elem_of_list_lookup;eauto. }
+    iDestruct (read_allowedU_inv _ x with "Hv") as "Hcond";auto. solve_addr.
+  Qed.
+
 
 End stack_object.
